Proved currency exchange external

proofs/currency_exchange_external.v
@@ -1,174 +1,176 @@
-Load helpers.
+Load metaproperties.
 
-Definition EXCHANGE_ADDR_EUR_TO_USD := 23.
-Definition exchange_office (timestamp : Time) := 
-  gateway EXCHANGE_ADDR_EUR_TO_USD 2 timestamp.
-
-
-Definition currency_exchange_gtw_desc
-           (amount : nat) :=
+(* ECX : External currency exchange *)
+Definition ecx_desc (addr : Address) (sc : nat) :=
   (And
-     (Give (Scale amount (One EUR)))
-     (ScaleObs EXCHANGE_ADDR_EUR_TO_USD (Scale amount (One USD)))
+     (Give (Scale sc (One EUR)))
+     (ScaleObs addr (Scale sc (One USD)))
   ).
 
-
-Definition exchange_ctr
-           (alice bob : Address)
-           (ctr_id dsc_id : Id)
-           (amount : nat) :=
-  finctr ctr_id
-         dsc_id
-         (currency_exchange_gtw_desc amount)
-         alice
-         bob
-         bob
-         1.
-
-Ltac exec_exchange H :=
-  match type of H with
-  | exec_ctr_in_state_with_owner (exchange_ctr _ _ _ _ _) _ _ = Some _ =>
-    unfold exchange_ctr, currency_exchange_gtw_desc, exec_ctr_in_state_with_owner in H; simpl in H; inversion H; clear H
-  end.
-
-
-Lemma exchange_alice_gets_paid_by_bob :
-  forall s1 alice bob ctr_id dsc_id result amount,
-    exec_ctr_in_state_with_owner
-      (exchange_ctr alice bob ctr_id dsc_id amount) s1 bob =
-    Some result ->
-    exists tr, # tr ∈ (res_ledger result) | ctr_id | bob --> alice | amount $ EUR #.
+(* The issuer pays the owner *)
+Lemma ecx_step_I_to_O:
+  forall s1 s2 ctr_id dsc_id addr sc amount I O ctr,
+    step s1 s2 ->
+    consistent_state s1 ->
+    ctr = finctr ctr_id dsc_id (ecx_desc addr amount) I O O sc ->
+    In ctr (m_contracts s1) ->
+    In (Executed ctr_id) (m_events s2) ->
+    O <> 0 ->
+    (exists obs tr,
+      In tr (m_ledger s2) /\
+      tr_ctr_id tr = ctr_id /\
+      tr_from tr = I /\
+      tr_to tr = O /\
+      tr_amount tr = sc * obs * amount).
 Proof.
   intros.
-  exec_exchange H.
-  case_eq (query (m_gateway s1) EXCHANGE_ADDR_EUR_TO_USD (m_global_time s1)); intros; rewrite H in H1; try inversion H1; clear H1.
-    eexists. simpl.
-    split.
-    + right. left. trivial.
-    + repeat split; trivial.
-      simpl. omega.
-Qed.
-      
-
-Lemma exchange_alice_gets_paid_by_bob_step :
-  forall s1 s2 alice bob ctr_id dsc_id amount,
-    In (exchange_ctr alice bob ctr_id dsc_id amount)  (m_contracts s1) ->
-    s1 → s2 ⊢ ctr_id ->
-    bob <> 0 ->
-    exists result tr,
-      # tr ∈ (res_ledger result) | ctr_id | bob --> alice | amount $ EUR #.
-Proof.
-  intros until 1.
-  step_intro.
-  assert (H' := H0); auto.
-  induction H0; intros; set (EX := (exchange_ctr alice bob ctr_id0 dsc_id0 amount)).
-  - unfold append_new_ctr_to_state in H8. subst s2. contradict_hyp H3.
-  - same_ctr ctr EX s2.
-    same_owner owner (ctr_owner EX) ctr EX.
-    subst ctr EX. subst owner. simpl in H9.
-    exists (result balance' ctrs' next' ledger').
-    eapply exchange_alice_gets_paid_by_bob.
-    exact H9.
-  - same_ctr ctr EX s2. subst ctr EX.
-    unfold exchange_ctr, currency_exchange_gtw_desc, ctr_primitive in H6. inversion H6.
-  - same_ctr ctr EX s2. subst ctr EX.
-    unfold exchange_ctr, currency_exchange_gtw_desc, ctr_primitive in H6. inversion H6.
-  - subst s2. contradict_hyp H3.
-  - subst s2. simpl in H3. contradiction.
+  induction H.
+  - subst s2. simpl in H3. destruct H3 as [H3 | H3]; try inversion H3.
+    apply consistent_impl_exec with (ctr := ctr) in H0; auto.
+    subst ctr. contradiction.
+  - case_eq (ctr_eq_dec ctr ctr0); intros; try contradiction.
+    unfold exec_ctr_in_state_with_owner in H10.
+    subst ctr0 ctr. simpl in H10.
+    case_match H10. destruct r. inversion H14. clear H14. subst.
+    case_eq (query (m_gateway s1) addr (m_global_time s1)); intros;
+      rewrite H10 in H1; inversion H1.
+    inversion H1. clear H1. simpl.
+    eexists. eexists. split. left. trivial.
+    simpl. repeat split; eauto.
+    destruct H5 as [H5 | H5]; simpl; subst; simpl; trivial. contradiction.
+  - case_eq (ctr_eq_dec ctr ctr0); intros; try contradiction.
+    subst ctr0. rewrite H1 in H7. unfold ecx_desc in H7.
+    simpl in H7. inversion H7.
+  - case_eq (ctr_eq_dec ctr ctr0); intros; try contradiction.
+    subst ctr0. rewrite H1 in H7. unfold ecx_desc in H7.
+    simpl in H7. inversion H7.
+  - case_eq (ctr_eq_dec ctr ctr0); intros; try contradiction.
+    subst ctr0 s2. simpl in H3.
+    destruct H3 as [H3 | H3]; try inversion H3.
+    apply consistent_impl_exec with (ctr := ctr) in H0; auto.
+    subst ctr. contradiction.
+  - subst s2. simpl in *.
+    apply consistent_impl_exec with (ctr := ctr) in H0; auto.
+    subst ctr. contradiction.
 Qed.
 
 
-Theorem exchange_alice_gets_paid_by_bob_steps :
-  forall s1 s2 alice bob ctr_id dsc_id amount,
-    In (exchange_ctr alice bob ctr_id dsc_id amount)  (m_contracts s1) ->
-    s1 ⇓ s2 ⊢ ctr_id ->
-    bob <> 0 ->
-    exists result tr,
-      # tr ∈ (res_ledger result) | ctr_id | bob --> alice | amount $ EUR #.
-Proof.
-  intros.
-  assert (H' := H); auto.
-  eapply exists_step_in_steps in H'; eauto.
-  destruct H' as [s [s' [H3' [H5' [H6' H7']]]]].
-  eapply exchange_alice_gets_paid_by_bob_step; eauto.
-Qed.
-
-
-Definition check_gateway (s : State) :=
-  query (m_gateway s) EXCHANGE_ADDR_EUR_TO_USD (m_global_time s).
-
-
-
-Lemma exchange_bob_gets_paid_by_alice :
-  forall s1 alice bob ctr_id dsc_id result amount rate,
-    exec_ctr_in_state_with_owner
-      (exchange_ctr alice bob ctr_id dsc_id amount) s1 bob = Some result ->
-    check_gateway s1 = Some rate ->
-    exists tr, # tr ∈ (res_ledger result) | ctr_id | alice --> bob | (rate * amount) $ USD #.
+Lemma ecx_steps_I_to_O:
+  forall s1 s2 ctr_id dsc_id addr sc amount I O ctr,
+    steps s1 s2 ->
+    consistent_state s1 ->
+    ctr = finctr ctr_id dsc_id (ecx_desc addr amount) I O O sc ->
+    In ctr (m_contracts s1) ->
+    In (Executed ctr_id) (m_events s2) ->
+    O <> 0 ->
+    (exists obs tr,
+      In tr (m_ledger s2) /\
+      tr_ctr_id tr = ctr_id /\
+      tr_from tr = I /\
+      tr_to tr = O /\
+      tr_amount tr = sc * obs * amount).
 Proof.
   intros.
-  exec_exchange H.
-  case_eq (query (m_gateway s1) EXCHANGE_ADDR_EUR_TO_USD (m_global_time s1)); intros; rewrite H in H2; try inversion H2; clear H2.
-    eexists. simpl.
-    split.
-    + left. trivial.
-    + repeat split; trivial.
-      simpl.
-      apply gateway_is_consistent with (t1 := (m_global_time s1))(v1 := rate) in H; auto.
-      subst. simpl.
-      rewrite Nat.add_0_r.
-      reflexivity.
+  induction H.
+  - subst. eapply consistent_impl_exec in H0; eauto.
+    simpl in *. contradiction.
+  - assert (H' := H).
+    apply steps_preserves_consistent_state in H'; auto.
+    apply steps_effect_over_contract with (ctr := ctr) in H; trivial.
+    destruct H as [H | [H | H]]; trivial.
+    + eapply ecx_step_I_to_O; eauto.
+    + subst ctr. simpl in *. eapply IHsteps in H.
+      destruct H as [obs [tr [H H'']]].
+      exists obs, tr. split; trivial.
+      eapply step_does_not_remove_transactions; eauto.
+    + eapply step_preserves_consistent_state in H'; eauto.
+      destruct H' as [_ [_ [_ [_ H']]]].
+      exfalso. eapply H'. subst ctr. simpl in *.
+      split; eauto.
+      eapply step_does_not_remove_events; eauto.
 Qed.
 
 
 
-Lemma exchange_bob_gets_paid_by_alice_step :
-  forall s1 s2 alice bob ctr_id dsc_id amount rate,
-    In (exchange_ctr alice bob ctr_id dsc_id amount)  (m_contracts s1) ->
-    s1 → s2 ⊢ ctr_id ->
-    bob <> 0 ->
-    check_gateway s1 = Some rate -> 
-    exists result tr,
-      # tr ∈ (res_ledger result) | ctr_id | alice --> bob | rate * amount $ USD #.
-Proof.
-  intros until 1.
-  step_intro.
-  assert (H' := H0); auto.
-  induction H0; intros; set (EX := (exchange_ctr alice bob ctr_id0 dsc_id0 amount)).
-  - unfold append_new_ctr_to_state in H8. subst s2. contradict_hyp H3.
-  - same_ctr ctr EX s2.
-    same_owner owner (ctr_owner EX) ctr EX.
-    subst EX ctr owner. simpl in H9.
-    exists (result balance' ctrs' next' ledger'). 
-    eapply exchange_bob_gets_paid_by_alice.
-    exact H9. auto.
-  - same_ctr ctr EX s2. subst ctr EX.
-    unfold exchange_ctr, currency_exchange_gtw_desc, ctr_primitive in H6. inversion H6.
-  - same_ctr ctr EX s2. subst ctr EX.
-    unfold exchange_ctr, currency_exchange_gtw_desc, ctr_primitive in H6. inversion H6.
-  - subst s2. contradict_hyp H3.
-  - subst s2. simpl in H3. contradiction.
-Qed.
-
-
-Theorem exchange_bob_gets_paid_by_alice_steps :
-  forall s1 s2 alice bob ctr_id dsc_id amount rate,
-    In (exchange_ctr alice bob ctr_id dsc_id amount)  (m_contracts s1) ->
-    s1 ⇓ s2 ⊢ ctr_id ->
-    bob <> 0 ->
-    check_gateway s1 = Some rate ->
-    gateway_stays_fresh s1 s2 ->
-    exists result tr,
-      # tr ∈ (res_ledger result) | ctr_id | alice --> bob | rate * amount $ USD #.
+(* The owner pays the issuer *)
+Lemma ecx_step_O_to_I:
+  forall s1 s2 ctr_id dsc_id addr sc amount I O ctr,
+    step s1 s2 ->
+    consistent_state s1 ->
+    ctr = finctr ctr_id dsc_id (ecx_desc addr amount) I O O sc ->
+    In ctr (m_contracts s1) ->
+    In (Executed ctr_id) (m_events s2) ->
+    O <> 0 ->
+    (exists tr,
+      In tr (m_ledger s2) /\
+      tr_ctr_id tr = ctr_id /\
+      tr_from tr = O /\
+      tr_to tr = I /\
+      tr_amount tr = sc * amount).
 Proof.
   intros.
-  assert (H' := H); auto.
-  eapply exists_step_in_steps in H'; eauto.
-  destruct H' as [s [s' [H3' [H5' [H6' H7']]]]].
-  eapply exchange_bob_gets_paid_by_alice_step; eauto.
-  unfold check_gateway in *.
-  eapply gateway_is_consistent_on_steps; eauto.
-  eapply gateway_stays_fresh_steps_left; eauto.
-  destruct H5' as [H5' H5''].
-  eapply tran_helper; eauto.
+  induction H.
+  - subst s2. simpl in H3. destruct H3 as [H3 | H3]; try inversion H3.
+    apply consistent_impl_exec with (ctr := ctr) in H0; auto.
+    subst ctr. contradiction.
+  - case_eq (ctr_eq_dec ctr ctr0); intros; try contradiction.
+    unfold exec_ctr_in_state_with_owner in H10.
+    subst ctr0 ctr. simpl in H10.
+    case_match H10. destruct r. inversion H14. clear H14. subst.
+    case_eq (query (m_gateway s1) addr (m_global_time s1)); intros;
+      rewrite H10 in H1; inversion H1.
+    inversion H1. clear H1. simpl.
+    eexists. split. right. left. trivial.
+    simpl. repeat split; eauto.
+    destruct H5 as [H5 | H5]; simpl; subst; simpl; trivial. contradiction.
+  - case_eq (ctr_eq_dec ctr ctr0); intros; try contradiction.
+    subst ctr0. rewrite H1 in H7. unfold ecx_desc in H7.
+    simpl in H7. inversion H7.
+  - case_eq (ctr_eq_dec ctr ctr0); intros; try contradiction.
+    subst ctr0. rewrite H1 in H7. unfold ecx_desc in H7.
+    simpl in H7. inversion H7.
+  - case_eq (ctr_eq_dec ctr ctr0); intros; try contradiction.
+    subst ctr0 s2. simpl in H3.
+    destruct H3 as [H3 | H3]; try inversion H3.
+    apply consistent_impl_exec with (ctr := ctr) in H0; auto.
+    subst ctr. contradiction.
+  - subst s2. simpl in *.
+    apply consistent_impl_exec with (ctr := ctr) in H0; auto.
+    subst ctr. contradiction.
+Qed.
+
+
+Lemma ecx_steps_O_to_I:
+  forall s1 s2 ctr_id dsc_id addr sc amount I O ctr,
+    steps s1 s2 ->
+    consistent_state s1 ->
+    ctr = finctr ctr_id dsc_id (ecx_desc addr amount) I O O sc ->
+    In ctr (m_contracts s1) ->
+    In (Executed ctr_id) (m_events s2) ->
+    O <> 0 ->
+    (exists tr,
+      In tr (m_ledger s2) /\
+      tr_ctr_id tr = ctr_id /\
+      tr_from tr = O /\
+      tr_to tr = I /\
+      tr_amount tr = sc * amount).
+Proof.
+  intros.
+  induction H.
+  - subst. eapply consistent_impl_exec in H0; eauto.
+    simpl in *. contradiction.
+  - assert (H' := H).
+    apply steps_preserves_consistent_state in H'; auto.
+    apply steps_effect_over_contract with (ctr := ctr) in H; trivial.
+    destruct H as [H | [H | H]]; trivial.
+    + eapply ecx_step_O_to_I; eauto.
+    + subst ctr. simpl in *. eapply IHsteps in H.
+      destruct H as [tr [H H'']].
+      exists tr. split; trivial.
+      eapply step_does_not_remove_transactions; eauto.
+    + eapply step_preserves_consistent_state in H'; eauto.
+      destruct H' as [_ [_ [_ [_ H']]]].
+      exfalso. eapply H'. subst ctr. simpl in *.
+      split; eauto.
+      eapply step_does_not_remove_events; eauto.
 Qed.
